pulse/lib/pulse_core/PulseCore.Memory.fst
@@ -1510,6 +1510,8 @@ let lift_h_exists #opened_invariants p = lift_tot_action (lift_heap_action opene
 
 let elim_pure #opened_invariants p = lift_tot_action (lift_heap_action opened_invariants (H.elim_pure p))
 
+let intro_pure #opened_invariants p pf = lift_tot_action (lift_heap_action opened_invariants (H.intro_pure p pf))
+
 let pts_to_join (#a:Type) (#pcm:pcm a) (r:ref a pcm) (x y : a) (m:mem) :
   Lemma (requires (interp (pts_to r x) m /\ interp (pts_to r y) m))
         (ensures (joinable pcm x y)) =
