pulse/lib/pulse_core/PulseCore.Action.fst
@@ -1,0 +1,191 @@
+module PulseCore.Action
+module Sem = PulseCore.Semantics2
+module Mem = PulseCore.Memory
+module I = PulseCore.InstantiatedSemantics
+open Mem
+open I
+
+let inames = Ghost.erased (FStar.Set.set iname)
+let emp_inames : inames = Ghost.hide Set.empty
+
+let join_inames (is1 is2 : inames) : inames =
+  Set.union is1 is2
+
+let inames_subset (is1 is2 : inames) : Type0 =
+  Set.subset is1 is2
+
+let (/!) (is1 is2 : inames) : Type0 =
+  Set.disjoint is1 is2
+
+unfold
+let inames_disj (ictx:inames) : Type = is:inames{is /! ictx}
+
+let act 
+    (a:Type u#a)
+    (opens:inames)
+    (pre:slprop)
+    (post:a -> slprop)
+= #ictx:inames_disj opens ->
+   action a ictx pre post
+
+let return 
+    (#a:Type u#a)
+    (#post:a -> slprop)
+    (x:a)
+: act a emp_inames (post x) post
+= fun #ictx -> return_action #a #ictx #post x
+
+let bind
+     (#a:Type u#a)
+     (#b:Type u#b)
+     (#opens:inames)
+     (#pre1 #post1 #post2:_)
+     (f:act a opens pre1 post1)
+     (g:(x:a -> act b opens (post1 x) post2))
+: act b opens pre1 post2
+= fun #ictx -> bind_action #a #b #ictx #pre1 #post1 #post2 (f #ictx) (fun x -> g x #ictx)
+
+let frame
+     (#a:Type u#a)
+     (#opens:inames)
+     (#pre #post #frame:_)
+     (f:act a opens pre post)
+: act a opens (pre `star` frame) (fun x -> post x `star` frame)
+= fun #ictx -> frame_action (f #ictx)
+
+let lift (#a:Type u#2) #opens #pre #post
+         (m:act a opens pre post)
+: stt a pre post
+= stt_of_action (m #emp_inames)
+
+let new_invariant (p:slprop)
+: act (inv p) emp_inames p (fun _ -> emp)
+= fun #ictx -> 
+    mem_action_as_action _ _ _ _ (new_invariant ictx p)
+
+let with_invariant
+    (#a:Type)
+    (#fp:slprop)
+    (#fp':a -> slprop)
+    (#f_opens:inames)
+    (#p:slprop)
+    (i:inv p{not (mem_inv f_opens i)})
+    (f:unit -> act a f_opens (p `star` fp) (fun x -> p `star` fp' x))
+: act a (add_inv f_opens i) fp fp'
+= fun #ictx ->
+    let ictx' = add_inv ictx i in
+    let f = action_as_mem_action _ _ _ _ (f () #ictx') in
+    let m = with_invariant i f in
+    mem_action_as_action _ _ _ _ m
+
+let weaken 
+    (#a:Type)
+    (#pre:slprop)
+    (#post:a -> slprop)
+    (#opens opens':inames)
+    (f:act a opens pre post)
+: act a (Set.union opens opens') pre post
+= f
+
+///////////////////////////////////////////////////////////////////
+// Core operations on references
+///////////////////////////////////////////////////////////////////
+open FStar.PCM
+open FStar.Ghost
+
+let ref (a:Type u#a) (p:pcm a) = ref a p
+
+let alloc
+    (#a:Type u#1)
+    (#pcm:pcm a)
+    (x:a{compatible pcm x x /\ pcm.refine x})
+: act (ref a pcm) emp_inames emp (fun r -> pts_to r x)
+= fun #ictx ->
+    mem_action_as_action _ _ _ _
+        (alloc_action ictx x)
+
+let read
+    (#a:Type)
+    (#p:pcm a)
+    (r:ref a p)
+    (x:erased a)
+    (f:(v:a{compatible p x v}
+        -> GTot (y:a{compatible p y v /\
+                     FStar.PCM.frame_compatible p x v y})))
+: act (v:a{compatible p x v /\ p.refine v}) emp_inames
+      (pts_to r x)
+      (fun v -> pts_to r (f v))
+= fun #ictx ->
+    mem_action_as_action _ _ _ _ (select_refine ictx r x f)
+
+let write
+    (#a:Type)
+    (#p:pcm a)
+    (r:ref a p)
+    (x y:Ghost.erased a)
+    (f:FStar.PCM.frame_preserving_upd p x y)
+: act unit emp_inames
+                  (pts_to r x)
+                  (fun _ -> pts_to r y)
+= fun #ictx -> mem_action_as_action _ _ _ _ (upd_gen ictx r x y f)
+
+let share
+    (#a:Type)
+    (#pcm:pcm a)
+    (r:ref a pcm)
+    (v0:FStar.Ghost.erased a)
+    (v1:FStar.Ghost.erased a{composable pcm v0 v1})
+: act unit emp_inames
+      (pts_to r (v0 `op pcm` v1))
+      (fun _ -> pts_to r v0 `star` pts_to r v1)
+= fun #ictx -> mem_action_as_action _ _ _ _ (split_action ictx r v0 v1)
+
+let gather
+    (#a:Type)
+    (#pcm:pcm a)
+    (r:ref a pcm)
+    (v0:FStar.Ghost.erased a)
+    (v1:FStar.Ghost.erased a)
+: act (squash (composable pcm v0 v1))
+    emp_inames
+    (pts_to r v0 `star` pts_to r v1)
+    (fun _ -> pts_to r (op pcm v0 v1))
+= fun #ictx -> mem_action_as_action _ _ _ _ (gather_action ictx r v0 v1)
+
+let witness
+    (#a:Type)
+    (#pcm:pcm a)
+    (r:erased (ref a pcm))
+    (fact:stable_property pcm)
+    (v:Ghost.erased a)
+    (pf:squash (forall z. compatible pcm v z ==> fact z))
+: act (witnessed r fact) emp_inames (pts_to r v) (fun _ -> pts_to r v)
+= fun #ictx -> mem_action_as_action _ _ _ _ (witness ictx r fact v pf)
+
+let recall
+    (#a:Type u#1)
+    (#pcm:pcm a)
+    (#fact:property a)
+    (r:erased (ref a pcm))
+    (v:Ghost.erased a)
+    (w:witnessed r fact)
+: act (v1:Ghost.erased a{compatible pcm v v1})
+    emp_inames
+    (pts_to r v)
+    (fun v1 -> pts_to r v `star` pure (fact v1))
+= fun #ictx -> mem_action_as_action _ _ _ _ (recall ictx r v w)
+
+///////////////////////////////////////////////////////////////////
+// pure
+///////////////////////////////////////////////////////////////////
+let intro_pure (p:prop) (pf:squash p)
+: act unit emp_inames emp (fun _ -> pure p)
+= fun #ictx -> mem_action_as_action _ _ _ _ (intro_pure #ictx p pf)
+
+let elim_pure (p:prop)
+: act (squash p) emp_inames (pure p) (fun _ -> emp)
+= fun #ictx -> mem_action_as_action _ _ _ _ (elim_pure #ictx p)
+
+///////////////////////////////////////////////////////////////////
+// exists*
+///////////////////////////////////////////////////////////////////
